# ðŸ“š Lecture 21: Eigenvalues and eigenvectors

**â—‹ Eigenvalues and eigenvectors**

$A\vec{v} = \lambda \vec{v} \quad (A\vec{v}$ is parallel to $\vec{v}$ and scaled by $\lambda)$

- <b>eigenvector</b> : $\vec{v}$<br>
A non-zero vector that has its direction unchanged by matrix $A$. ($A$ : Given linear transformation<br>
<b>Only changes in magnitude</b> by corresponding eigenvalue $lambda$.

- <b>eigenvalue</b> : $\lambda$<br>
The scalar by which the corresponding eigenvector is scaled.
<br><br>

**â—‹ How to find $(\lambda, \vec{v})$ pairs from $A\vec{v} = \lambda \vec{v}$ ?**<br>
- From $\quad [A\vec{v} = \lambda \vec{v} \quad\leftrightarrow\quad (A - \lambda I)\vec{v} = \vec{0}$],<br>
$(A - \lambda I)$ must be <b>singular</b>.<br>
$\therefore \det (A - \lambda I) = 0$
<br><br>

**â—‹ Properties**<br>

- If $A$ is <b>singular</b>, then at least one of $\lambda = 0$.

- What is the $(\lambda, \vec{v})$ for a projection matrix $P$?<br>
Any $\vec{v}$ in the plane : $P\vec{v} = \vec{v} \quad (\lambda = 1)$

- Permutation matrix

```math
\begin{align}
A = \begin{bmatrix} 0 & 1 \\ 1 & 0 \end{bmatrix} \quad\text{(exchange row1 and row2)} \\
(\lambda_{1}, \vec{v}_{1}) = (1, \begin{bmatrix} 1 \\ 1 \end{bmatrix}) \quad\rightarrow\quad \begin{bmatrix} 0 & 1 \\ 1 & 0 \end{bmatrix}\begin{bmatrix} 1 \\ 1 \end{bmatrix} = \begin{bmatrix} 1 \\ 1 \end{bmatrix} \\
(\lambda_{2}, \vec{v}_{2}) = (-1, \begin{bmatrix} -1 \\ 1 \end{bmatrix}) \quad\rightarrow\quad \begin{bmatrix} 0 & 1 \\ 1 & 0 \end{bmatrix}\begin{bmatrix} -1 \\ 1 \end{bmatrix} = -\begin{bmatrix} -1 \\ 1 \end{bmatrix} \\
\end{align}
```
<br>

- (Sum of the eigenvalues) = (Sum of the diagonal entries)
```math
\begin{align}
\det (\lambda I - A) = \begin{cases}
\lambda^{n} - (a_{11}+a_{22}+\cdots+a_{nn})\lambda^{n-1} + \cdots = 0 \\
(\lambda-\lambda_{1})(\lambda-\lambda_{2})\cdots(\lambda-\lambda_{n}) = \lambda^{n} - (\lambda_{1}+\lambda_{2}+\cdots+\lambda_{n})\lambda^{n-1} + \cdots = 0 \end{cases} \\
\therefore \: \text{tr}(A) = \sum_{i=1}^{n} a_{ii} = a_{11} + a_{22} + \cdots + a_{nn} \\
 = \lambda_{1} + \lambda_{2} + \cdots + \lambda_{n} = \sum_{i=1}^{n} \lambda_{i}
\end{align}
```
<br>

- In case of $A\prime = A + kI$, (where $k$ is constant)
```math
\begin{align}
A\prime\vec{v}\prime = (A + kI)\vec{v}\prime = A\vec{v}\prime + k\vec{v}\prime = \lambda\prime\vec{v}\prime \\
A\vec{v}\prime = (\lambda\prime - k)\vec{v}\prime = \lambda\vec{v} \\
\therefore \: (\lambda, \vec{v}) = (\lambda\prime-k, \vec{v}\prime) \quad\leftrightarrow\quad (\lambda\prime, \vec{v}\prime) = (\lambda+k, \vec{v})
\end{align}
```
<br>

Example)
```math
A\prime = \begin{bmatrix} 3 & 1 \\ 1 & 3 \end{bmatrix} = \begin{bmatrix} 0 & 1 \\ 1 & 0 \end{bmatrix} + \begin{bmatrix} 3 & 0 \\ 0 & 3 \end{bmatrix} = A + 3I
```
```math
\begin{align}
\det (A\prime - \lambda\prime I) {} &= \begin{vmatrix} 3-\lambda\prime & 1 \\ 1 & 3-\lambda\prime \end{vmatrix} \\\\
&= (3-\lambda\prime)^{2} - 1 \\\\
&= \lambda\prime^{2} - 6\lambda\prime + 8 \\\\
&= (\lambda\prime-4)(\lambda\prime-2)
\end{align}
```
<br>

```math
\begin{align} (\lambda\prime, \vec{v}\prime) = \begin{cases}
(\lambda\prime_{1}, \vec{v}\prime_{1}) = (4, \begin{bmatrix} 1 \\ 1 \end{bmatrix}) \\
(\lambda\prime_{2}, \vec{v}\prime_{2}) = (2, \begin{bmatrix} -1 \\ 1 \end{bmatrix})
\end{cases} \quad\leftrightarrow\quad
(\lambda, \vec{v}) = (\lambda\prime-3, \vec{v}\prime) = \begin{cases} (1, \begin{bmatrix} 1 \\ 1 \end{bmatrix}) \\ (-1, \begin{bmatrix} -1 \\ 1 \end{bmatrix})
\end{cases}
\end{align}
```
<br>

- 90Âº Rotation matrix $Q$ (orthogonal)

```math
\begin{align}
Q = \begin{bmatrix} 0 & -1 \\ 1 & 0 \end{bmatrix} \\
trace = 0 + 0 = \lambda_{1} + \lambda_{2} \\
det = 1 = \lambda_{1}\lambda_{2}
\end{align}
```

```math
\begin{align}
\det (Q - \lambda I) = \begin{vmatrix} -\lambda & -1 \\ 1 & -\lambda \end{vmatrix}  = \lambda^{2} + 1 = (\lambda-i)(\lambda+i) = 0 \\
\lambda_{1} = i, \vec{v}_{1} = \begin{bmatrix} i \\ 1 \end{bmatrix} \\
\lambda_{2} = -i, \vec{v}_{2} = \begin{bmatrix} i \\ -1 \end{bmatrix}
\end{align}
```

- Triangular Matrix

```math
\begin{align}
A = \begin{bmatrix} 3 & 1 \\ 0 & 3 \end{bmatrix} \\

\det (A - \lambda I) = \begin{vmatrix} 3-\lambda & 1 \\ 0 & 3-\lambda \end{vmatrix}  = (3-\lambda)^{2} \\
\lambda_{1} = \lambda_{2} = 3, \vec{v}_{1} = \begin{bmatrix} 1 \\ 0 \end{bmatrix} \\
\text{No 2nd independent} \: \vec{v}_{2}
\end{align}
```

<br><br><br>

# ðŸ“š Lecture 22: Diagonalization and powers of A

**â—‹ Eigenvalues and eigenvectors**



Suppose $n$ independent eigenvectors of $A$.
Put them in columns.

```math
\begin{align}
AS {} &= A \begin{bmatrix} \vec{v}_{1} & \vec{v}_{2} & \cdots & \vec{v}_{n} \end{bmatrix} \\
&= \begin{bmatrix} \lambda_{1}\vec{v}_{1} & \lambda_{2}\vec{v}_{2} & \cdots & \lambda_{n}\vec{v}_{n} \end{bmatrix} \\
&= \begin{bmatrix} \vec{v}_{1} & \vec{v}_{2} & \cdots & \vec{v}_{n} \end{bmatrix} \begin{bmatrix}
\lambda_{1} & 0 & \cdots & 0 \\
0 & \lambda_{2} & \cdots & 0 \\
\vdots & \vdots & \ddots & \vdots \\
0 & 0 & \cdots & \lambda_{n}
\end{bmatrix} \\
&= S\Lambda
\end{align}
```
<br>

```math
\therefore \: S^{-1}AS = \Lambda \quad\leftrightarrow\quad S\Lambda S^{-1} = A
```

If A\vec{v} = \lambda \vec{v} ,
A^{2}\vec{v} = A(\lambda \vec{v}) = \lambda (A\vec{v}) = \lambda^{2}\vec{v}

A^{2} = (S\Lambda S^{-1})(S\Lambda S^{-1}) = S\Lambda^{2} S^{-1}
A^{k} = S\Lambda^{k} S^{-1}
eigenvalues of A^{k} are the k-th powers of the eigenvalues of A.
eigenvectors of A^{k} are the same of the eigenvectors of A.

Theorem
A^{k} \rightarrow 0 as k \rightarrow \inf
if all |\lambda_{i}| < 1

Assumption
We have full set of n independent eigenvectors. (= S is invertible)
If not, we can't diagonalize the matrix.

$A$ is sure to have $n$ independent eigenvectors (and be diagonalizeable)
if all the $\lambda$'s are different (no repeated $\lambda$'s)

Repeated eigenvalues : May or may not have n independent eigenvectors.

Example) In this case, need 2 independent eigenvectors to have S^{-1},  but only one eigenvalue and one eigenvector exist.

```math
\begin{align}
A = \begin{bmatrix} 2 & 1 \\ 0 & 2 \end{bmatrix} \\
\det(A- \lambda I) = \begin{vmatrix} 2-\lambda & 1 \\ 0 & 2-\lambda \end{vmatrix} = (2-\lambda)^{2} = 0 \\
(\lambda_{1}, \vec{v}_{1}) = (2, \begin{bmatrix} 1 \\ 0 \end{bmatrix})
\end{align}
```