# ðŸ“š Lecture 23: Differential equations and exp(At)

**â—‹ Differential Equations**

For time variable $t$,

```math
\begin{align}
\text{For}\quad \vec{u}(t) = \begin{bmatrix} u_{1}(t) \\ u_{2}(t) \end{bmatrix} \quad\text{,}\quad \vec{u}(0) = \begin{bmatrix} u_{1}(0) \\ u_{2}(0) \end{bmatrix} = \begin{bmatrix} 1 \\ 0 \end{bmatrix} \\

\text{and}\quad \frac{d\vec{u}}{dt} = \begin{bmatrix} \frac{du_{1}}{dt} \\ \frac{du_{2}}{dt} \end{bmatrix} = \begin{bmatrix} -u_{1} + 2u_{2} \\ u_{1} - 2u_{2} \end{bmatrix} = \begin{bmatrix} -1 & 2 \\ 1 & -2 \end{bmatrix} \begin{bmatrix} u_{1} \\ u_{2} \end{bmatrix} \\

\text{â†’ Solve Differential Equations}\quad \frac{d\vec{u}}{dt} = A\vec{u} \quad\text{for}\quad A = \begin{bmatrix} -1 & 2 \\ 1 & -2 \end{bmatrix}
\end{align}
```

```math
\begin{align}
{} & \text{Eigenvalues of}\: A \: \text{:}\quad\begin{cases}
\lambda_{1} = 0 \quad(\because A \: \text{is singular}) \\
\lambda_{2} = -3 \quad(\because tr(A) = \lambda_{1} + \lambda_{2} = -3)
\end{cases} \\
& \text{Eigenvectors of}\: A \: \text{:}\quad\begin{cases}
(\lambda_{1},\vec{v}_{1}) = (0,\begin{bmatrix} 2 \\ 1 \end{bmatrix}) \\
(\lambda_{2},\vec{v}_{2}) = (-3,\begin{bmatrix} 1 \\ -1 \end{bmatrix}) \end{cases}
\end{align}
```

```math
\begin{align}
\text{Solution :}\quad \vec{u}(t) {} &= c_{1}e^{\lambda_{1}t}\vec{v}_{1} + c_{2}e^{\lambda_{2}t}\vec{v}_{2} \\
&= c_{1}e^{0t}\begin{bmatrix} 2 \\ 1 \end{bmatrix} + c_{2}e^{-3t}\begin{bmatrix} 1 \\ -1 \end{bmatrix} \\
&= c_{1}\begin{bmatrix} 2 \\ 1 \end{bmatrix} + c_{2}e^{-3t}\begin{bmatrix} 1 \\ -1 \end{bmatrix} \\
&= \frac{1}{3}\begin{bmatrix} 2 \\ 1 \end{bmatrix} + \frac{1}{3}e^{-3t}\begin{bmatrix} 1 \\ -1 \end{bmatrix}
\end{align}
```

```math
\begin{cases}
\because\: \vec{u}(0) {} &= c_{1}\vec{v}_{1} + c_{2}\vec{v}_{2} \\
&= c_{1}\begin{bmatrix} 2 \\ 1 \end{bmatrix} + c_{2}\begin{bmatrix} 1 \\ -1 \end{bmatrix} \\
&= S\vec{c} = \begin{bmatrix} 2 & 1 \\ 1 & -1 \end{bmatrix} \begin{bmatrix} c_{1} \\ c_{2} \end{bmatrix} = \begin{bmatrix} 1 \\ 0 \end{bmatrix} \\
\quad\therefore\: \vec{c} &= S^{-1}\vec{u}(0) = \begin{bmatrix} \frac{1}{3} & \frac{1}{3} \\ \frac{1}{3} & -\frac{2}{3} \end{bmatrix} \begin{bmatrix} 1 \\ 0 \end{bmatrix} = \begin{bmatrix} \frac{1}{3} \\ \frac{1}{3} \end{bmatrix}
\end{cases}
```
<br>

```math
\begin{align}
\text{For}\quad \vec{u}(t) = \frac{1}{3}\begin{bmatrix} 2 \\ 1 \end{bmatrix} + \frac{1}{3}e^{-3t}\begin{bmatrix} 1 \\ -1 \end{bmatrix}\: , \\
\text{as}\quad t\to\infty \quad\text{then}\: \lim_{k\to\infty} \vec{u}(t) \approx \frac{1}{3}\begin{bmatrix} 2 \\ 1 \end{bmatrix} \quad\text{(Steady State)}
\end{align}
```
<br>

As $t\to\infty$,<br>
â‘  Stability $(\vec{u}(t) \to 0)$<br>
$\quad$ Condition : All $\Re(\lambda) < 0 \quad(\leftrightarrow tr(A) = \lambda_{1}+\lambda_{2} < 0$ and $det(A) = \lambda_{1}\lambda_{2} > 0)$<br>
â‘¡ Steady State $(\vec{u}(t) \to const.)$<br>
$\quad$ Condition : $\lambda_{1} = 0$ and $\Re(\lambda_{2}) < 0$<br>
â‘¢ Blow up if any $\Re(\lambda) > 0$<br>


Matrix Exponential

e^{At}